src/Canonical_form.v
@@ -1,0 +1,42 @@
+From Coq Require Import Unicode.Utf8.
+Require Import ZArith.
+Local Open Scope Z_scope.
+Require Import Syntax.
+Require Import Types.
+Require Import Hints.
+
+Local Lemma t_num : ∀ e,
+    has_type empty e Type_Num -> 
+    value e ->
+    ∃ z, e = E_Num z.
+Proof.
+    intros * H_type H_val.
+    inversion H_val; eauto; 
+    subst; inversion H_type.
+Qed.
+
+Hint Resolve t_num : local_hints.
+
+Local Lemma t_bool : ∀ e,
+    has_type empty e Type_Bool -> 
+    value e ->
+    e = E_True \/ e = E_False.
+Proof.
+    intros * H_type H_val.
+    inversion H_val; subst; auto;
+    inversion H_type.
+Qed.
+
+Hint Resolve t_bool : local_hints.
+
+Local Lemma t_fun : ∀ e t1 t2,
+    has_type empty e (Type_Fun t1 t2) -> 
+    value e ->
+    ∃ x e', e = E_Fun x t1 e'. 
+Proof.
+    intros * H_type H_val.
+    inversion H_val; subst; try (inversion H_type; fail).
+    inversion H_type; subst.
+    eauto.
+Qed.
+Hint Resolve t_fun : local_hints.
