src/Progress.v
@@ -1,0 +1,52 @@
+From Coq Require Import Unicode.Utf8.
+From Coq Require Import Strings.String.
+Require Import Maps.
+Local Open Scope Z_scope.
+Require Import ZArith.
+Require Import Syntax.
+Require Import Subst.
+Require Import Step.
+Require Import Types.
+Require Import Free.
+Require Import Canonical_form.
+Require Import Hints.
+
+
+Print HintDb local_hints.
+
+
+Theorem expr_progress : ∀ e t,
+    has_type empty e t -> 
+    value e \/ ∃ e', step e e'.
+Proof with eauto with local_hints.
+    intros * H_type.
+    generalize dependent t.
+    induction e; intros;
+    try (eauto with local_hints; fail);
+    (right; inversion H_type; subst)...
+
+    - inversion H1.
+
+    - destruct (IHe1 (Type_Fun t1 t)) as [H_val_e1 | [e1' H_step_e1] ]...
+      destruct (IHe2 t1) as [H_val_e2 | [e2' H_step_e2] ]...
+      destruct (Canonical_form.t_fun e1 t1 t H4 H_val_e1) as [x [e' H_eq]]; subst.
+      destruct (IHe1 _ H4) as [H_val | H_ex];
+      [ destruct (Subst.exists_one e2 x e') as [e'0 H_sub] 
+      | destruct H_ex as [e'0 H_ex]]...
+
+    - destruct (IHe1 _ H3) as [H_val_e1 | [e' H_step]]...
+      apply Canonical_form.t_bool in H_val_e1...
+      destruct H_val_e1 as [H_e1_eq | H_e1_eq]; subst...
+
+    - destruct (IHe1 t1) as [H_val_e1 | [e1' H_step_e1] ]...
+      destruct (Subst.exists_one e1 x e2) as [e' H_sub]...
+    
+    - apply IHe1 in H2 as He1. apply IHe2 in H4 as He2.
+      destruct He1 as [H_v_e1 | [e1' H_step_e1]]...
+      destruct He2 as [H_v_e2 | [e2' H_step_e2]]...
+      destruct (Canonical_form.t_num e1 H2 H_v_e1) as [z1 H_z1].
+      destruct (Canonical_form.t_num e2 H4 H_v_e2) as [z2 H_z2].
+      subst...
+Qed.
+
+Hint Resolve expr_progress : local_hints.
