src/Subst.v
@@ -1,0 +1,70 @@
+From Coq Require Import Unicode.Utf8.
+From Coq Require Import Strings.String.
+Local Open Scope Z_scope.
+Require Import ZArith.
+Require Import Syntax.
+Require Import Hints.
+
+Inductive substitution (s : expr) (x : string) : expr -> expr -> Prop :=
+    | S_Var_Eq :
+        substitution s x (E_Var x) s
+    | S_Var_Neq :
+        forall (y : string), x <> y -> substitution s x (E_Var y) (E_Var y)
+    | S_App : 
+        forall (e1 e1' e2 e2' : expr),
+        substitution s x e1 e1' ->
+        substitution s x e2 e2' ->
+        substitution s x (E_App e1 e2) (E_App e1' e2')
+    | S_Fun_Eq : 
+        forall (t : type) (e : expr),
+        substitution s x (E_Fun x t e) (E_Fun x t e)
+    | S_Fun_Neq : 
+        forall (y : string) (t : type) (e e' : expr),
+        x <> y -> substitution s x e e' -> 
+        substitution s x (E_Fun y t e) (E_Fun y t e')
+    | S_True : 
+        substitution s x E_True E_True
+    | S_False : 
+        substitution s x E_False E_False
+    | S_If : 
+        forall (e1 e1' e2 e2' e3 e3' : expr),
+        substitution s x e1 e1' ->
+        substitution s x e2 e2' ->
+        substitution s x e3 e3' ->
+        substitution s x (E_If e1 e2 e3) (E_If e1' e2' e3')
+    | S_Let_Eq : 
+        forall (e1 e1' e2: expr),
+        substitution s x e1 e1' -> 
+        substitution s x (E_Let x e1 e2) (E_Let x e1' e2)
+    | S_Let_Neq : 
+        forall (y : string) (e1 e1' e2 e2': expr),
+        x <> y ->
+        substitution s x e1 e1' -> 
+        substitution s x e2 e2' -> 
+        substitution s x (E_Let y e1 e2) (E_Let y e1' e2')
+    | S_Num : 
+        forall (z : Z),
+        substitution s x (E_Num z) (E_Num z)
+    | S_Minus :
+        forall (e1 e1' e2 e2': expr),
+        substitution s x e1 e1' -> 
+        substitution s x e2 e2' -> 
+        substitution s x (E_Minus e1 e2) (E_Minus e1' e2')
+.
+
+Hint Constructors substitution : local_hints.
+
+Local Lemma exists_one : ∀ s x e, ∃ e', substitution s x e e'.
+Proof with eauto.
+    intros.
+    induction e;
+    try destruct IHe;
+    try destruct IHe1;
+    try destruct IHe2; 
+    try destruct IHe3; 
+    try destruct (String.eqb_spec x x0); 
+    subst;
+    eauto with local_hints.
+Qed.
+
+Hint Resolve exists_one : local_hints.
