src/Syntax.v
@@ -1,0 +1,41 @@
+From Coq Require Import Unicode.Utf8.
+From Coq Require Import Strings.String.
+Local Open Scope Z_scope.
+Require Import ZArith.
+Require Import Hints.
+
+Inductive type :=
+| Type_Num
+| Type_Bool
+| Type_Fun (e1 e2 : type) : type
+.
+
+
+Inductive expr := 
+| E_Var (x : string) 
+| E_App (e1 e2 : expr) 
+| E_Fun (x : string) (t : type) (e : expr) 
+| E_True  
+| E_False 
+| E_If (e1 e2 e3 : expr)  
+| E_Let (x : string) (e1 e2 : expr)
+| E_Num (z : Z)
+| E_Minus (e1 e2 : expr)
+.
+
+
+Inductive value : expr -> Prop :=
+| V_Num : forall z, value (E_Num z)
+| V_True : value E_True
+| V_False : value E_False
+| V_Fun : 
+    forall 
+        (x : string) 
+        (t : type) 
+        (e : expr), 
+    value (E_Fun x t e)
+.
+
+Hint Constructors type : local_hints.
+Hint Constructors expr : local_hints.
+Hint Constructors value : local_hints.
