src/Types.v
@@ -1,0 +1,78 @@
+From Coq Require Import Unicode.Utf8.
+From Coq Require Import Strings.String.
+Local Open Scope Z_scope.
+Require Import ZArith.
+Require Import Maps.
+Require Import Syntax.
+Require Import Step.
+Require Import Hints.
+
+Definition context := @Maps.map type.
+Definition empty := @Maps.empty type.
+
+
+Inductive has_type : context -> expr -> type -> Prop := 
+| T_Var: forall Γ x t, 
+            Γ ? x = Some t -> 
+            has_type Γ (E_Var x) t
+
+| T_Fun: forall Γ x t1 e t2,
+            has_type (x |-> t1; Γ) e t2 ->
+            has_type Γ (E_Fun x t1 e) (Type_Fun t1 t2)
+| T_App: forall Γ e1 e2 t1 t2, 
+            has_type Γ e2 t1 -> 
+            has_type Γ e1 (Type_Fun t1 t2) ->
+            has_type Γ (E_App e1 e2) t2
+
+| T_True: forall Γ, 
+            has_type Γ E_True Type_Bool
+| T_False: forall Γ, 
+            has_type Γ E_True Type_Bool
+
+| T_If: forall Γ e1 e2 e3 t, 
+            has_type Γ e1 Type_Bool -> 
+            has_type Γ e2 t -> 
+            has_type Γ e3 t -> 
+            has_type Γ (E_If e1 e2 e3) t 
+| T_Let : forall Γ x e1 e2 t1 t2, 
+            has_type Γ e1 t1 -> 
+            has_type (x |-> t1; Γ) e2 t2 -> 
+            has_type Γ (E_Let x e1 e2) t2
+| T_Num : forall Γ z, has_type Γ (E_Num z) Type_Num 
+| T_Minus : forall Γ e1 e2, 
+              has_type Γ e1 Type_Num ->
+              has_type Γ e2 Type_Num ->
+              has_type Γ (E_Minus e1 e2) Type_Num 
+.
+
+Hint Constructors has_type : local_hints.
+
+
+Local Lemma weakening : ∀ Γ Γ' e t, 
+    includedin Γ Γ' ->
+    has_type Γ e t ->
+    has_type Γ' e t.
+Proof.
+    intros * H_included H_type.
+    generalize dependent Γ'.
+    induction H_type; intros; eauto with local_hints.
+    - apply T_Fun. apply IHH_type.
+      apply Maps.includedin_update. assumption.
+    - eapply T_Let; eauto. 
+      apply IHH_type2.
+      apply Maps.includedin_update.
+      assumption.
+Qed.
+
+Hint Resolve weakening : local_hints.
+
+
+Lemma weakening_empty : ∀ Γ e t, 
+    has_type empty e t ->
+    has_type Γ e t.
+Proof.
+intros. apply (weakening empty); auto.
+intros x v contra. discriminate contra.
+Qed.
+
+Hint Resolve weakening_empty : local_hints.
