src/Hints.v
@@ -1,0 +1,1 @@
+Create HintDb local_hints.
